bunch of stuff, a bit messy

theories/backtranslation/cast_help/between.v
@@ -3,6 +3,16 @@ From fae_gtlc_mu Require Export prelude.
 
 (** Between sums, products, recursive types, arrow types *)
 
+Lemma subst_lam e σ : (Lam e).[σ] = Lam e.[up σ].
+Proof.
+  by simpl.
+Qed.
+
+Lemma subst_app e1 e2 σ : (App e1 e2).[σ] = (App e1.[σ] e2.[σ]).
+Proof.
+  by simpl.
+Qed.
+
 Definition between_TSum (c1 c2 : expr) : expr :=
   Lam (Case (Var 0) (InjL ((rename (+2) c1) (Var 0))) (InjR ((rename (+2) c2) (Var 0)))).
 
@@ -40,6 +50,14 @@ Definition between_TArrow (ca cr : expr) : expr :=
        )
     ).
 
+Lemma between_TArrow_subst_rewrite σ ca cr :
+  (between_TArrow ca cr).[σ] =
+  between_TArrow ca.[σ] cr.[σ].
+Proof.
+  rewrite /between_TArrow.
+  by asimpl.
+Qed.
+
 Lemma between_TArrow_typed Γ (τ1 τ2 τ3 τ4 : type) (ca cr : expr) (da : Γ ⊢ₛ ca : (TArrow τ3 τ1)) (dr : Γ ⊢ₛ cr : (TArrow τ2 τ4)) :
   Γ ⊢ₛ between_TArrow ca cr : (TArrow (TArrow τ1 τ2) (TArrow τ3 τ4))%type.
 Proof.
@@ -70,7 +88,8 @@ Proof.
   apply App_typed with (τ1 := TRec τi).
   (* apply App_typed with (τ1 := ((TRec τi → TRec τf) → (TRec τi → TRec τf))). *)
   eapply App_typed.
-  apply Fix_typed; by intro τ; simpl; rewrite -(Pi τ); rewrite -(Pf τ); by simpl.
+  apply Fix_typed; auto.
+    (* by intro τ; simpl; rewrite -(Pi τ); rewrite -(Pf τ); by simpl. *)
   apply Lam_typed.
   apply Lam_typed.
   apply Fold_typed.
@@ -85,3 +104,126 @@ Proof.
   by apply Var_typed.
   by apply Var_typed.
 Qed.
+
+Definition between_TRec' (f : expr) : expr :=
+  Lam (* x : μ. τi *) (
+      Fix'' (
+          Lam (* g : μ.τi → μ.τf *) (
+              Lam (* r : μ.τi *) (
+                  Fold (rename (+1) (f.[upn 1 (ren (+ 1))])(* : τi.[μ.τi/] → τf.[μ.τf]*) (Unfold (Var 0)))
+                )
+            )
+        ) (Var 0)
+    ).
+
+Lemma between_TRec'_subst_rewrite σ f :
+  (between_TRec' f).[σ] =
+  between_TRec' f.[up σ].
+Proof.
+  rewrite /between_TRec'.
+  rewrite subst_lam.
+  rewrite subst_app.
+  rewrite Fix''_subs_rewrite.
+  by asimpl.
+Qed.
+
+Definition between_TRecV' (f : expr) : val :=
+  LamV (* x : μ. τi *) (
+      Fix'' (
+          Lam (* g : μ.τi → μ.τf *) (
+              Lam (* r : μ.τi *) (
+                  Fold (rename (+1) (f.[upn 1 (ren (+ 1))])(* : τi.[μ.τi/] → τf.[μ.τf]*) (Unfold (Var 0)))
+                )
+            )
+        ) (Var 0)
+    ).
+
+Lemma between_TRec'_to_value f : between_TRec' f = stlc_mu.lang.of_val (between_TRecV' f).
+Proof.
+  by simpl.
+Qed.
+
+Lemma between_TRec'_typed Γ (τi τf : type) (Pi : Is_Closed (TRec τi)) (Pf : Is_Closed (TRec τf)) (f : expr)
+      (d : ((TArrow (TRec τi) (TRec τf)):: Γ) ⊢ₛ f : (TArrow (τi.[TRec τi/]) τf.[TRec τf/])) :
+  Γ ⊢ₛ between_TRec' f : (TArrow (stlc_mu.typing.TRec τi) (stlc_mu.typing.TRec τf))%type.
+Proof.
+  apply Lam_typed.
+  apply App_typed with (τ1 := TRec τi).
+  apply Fix''_typed; auto.
+    (* by intro τ; simpl; rewrite -(Pi τ); rewrite -(Pf τ); by simpl. *)
+  apply Lam_typed.
+  apply Lam_typed.
+  apply Fold_typed.
+  apply App_typed with (τ1 := τi.[(TRec τi)/]).
+  apply up_type_one.
+  rewrite rewrite_for_context_weakening in d.
+  rewrite (rewrite_for_context_weakening Γ).
+  rewrite rewrite_for_context_weakening.
+  apply context_gen_weakening.
+  apply d.
+  apply Unfold_typed.
+  by apply Var_typed.
+  by apply Var_typed.
+Qed.
+
+Definition between_TRec_stepped (f : expr) : expr :=
+  Lam (* x : μ. τi *) (
+      Fix_stepped.[(
+          Lam (* g : μ.τi → μ.τf *) (
+              Lam (* r : μ.τi *) (
+                  Fold (rename (+1) (f.[upn 1 (ren (+ 1))])(* : τi.[μ.τi/] → τf.[μ.τf]*) (Unfold (Var 0)))
+                )
+            )
+        )/] (Var 0)
+    ).
+
+Lemma between_TRec_stepped_typed Γ (τi τf : type) (Pi : Is_Closed (TRec τi)) (Pf : Is_Closed (TRec τf)) (f : expr)
+      (d : ((TArrow (TRec τi) (TRec τf)):: Γ) ⊢ₛ f : (TArrow (τi.[TRec τi/]) τf.[TRec τf/])) :
+  Γ ⊢ₛ between_TRec_stepped f : (TArrow (stlc_mu.typing.TRec τi) (stlc_mu.typing.TRec τf))%type.
+Proof.
+  apply Lam_typed.
+  apply App_typed with (τ1 := TRec τi).
+  apply Fix_stepped_subs_typed; auto.
+    (* by intro τ; simpl; rewrite -(Pi τ); rewrite -(Pf τ); by simpl. *)
+  apply Lam_typed.
+  apply Lam_typed.
+  apply Fold_typed.
+  apply App_typed with (τ1 := τi.[(TRec τi)/]).
+  apply up_type_one.
+  rewrite rewrite_for_context_weakening in d.
+  rewrite (rewrite_for_context_weakening Γ).
+  rewrite rewrite_for_context_weakening.
+  apply context_gen_weakening.
+  apply d.
+  apply Unfold_typed.
+  by apply Var_typed.
+  by apply Var_typed.
+Qed.
+
+(* Lemma between_TRec_subs (f : expr) σ : (between_TRec_stepped f).[σ] = between_TRec_stepped (f.[ids 0 .: σ]). *)
+(* Proof. *)
+(*   rewrite /between_TRec_stepped /Fix_stepped. *)
+(*   asimpl. *)
+(*   auto. *)
+(*   repeat rewrite rename_ren. *)
+(*   simpl. *)
+(*   f_equal. *)
+(*   f_equal. *)
+(*   f_equal. *)
+(*   f_equal. *)
+(*   f_equal. *)
+(*   f_equal. *)
+(*   f_equal. *)
+(*   repeat rewrite subst_comp. repeat rewrite up_lift1. asimpl. *)
+(*   rewrite -fold_ren_cons *)
+
+
+(*   admit. *)
+(*   asimpl. *)
+(*   asimpl. *)
+(*   asimpl. *)
+(*   repeat f_equal. *)
+(*   asimpl.  *)
+(*   rewrite /up. *)
+(*   rewrite -up_comp. *)
+(*   asimpl. *)
