theories/stlc_mu/lib/fix.v
@@ -1,31 +1,201 @@
 From fae_gtlc_mu Require Export stlc_mu.lang.
 From fae_gtlc_mu Require Export stlc_mu.typing.
 
-Coercion App : expr >-> Funclass.
-(* Infix "→" := TArrow : type_scope. *)
-
 Definition Fix : expr :=
   Lam (
-      (Lam (Var 1 ((Unfold (Var 0)) (Var 0))))
-        (Fold (Lam (Var 1 ((Unfold (Var 0)) (Var 0)))))
+      (Lam (Var 1 (Lam ((Unfold (Var 1)) (Var 1) (Var 0)))))
+        (Fold (Lam (Var 1 (Lam ((Unfold (Var 1)) (Var 1) (Var 0))))))
   ).
 
-Definition Fix_typed Γ τ : (Is_Closed τ) -> (Γ ⊢ₛ Fix : (TArrow (TArrow τ τ) τ)).
+Definition Fix_typed Γ τa τr (pa : Is_Closed τa) (pr : Is_Closed τr) :
+  (Γ ⊢ₛ Fix : (TArrow (TArrow (TArrow τa τr) (TArrow τa τr)) (TArrow τa τr))).
 Proof.
-  intro P.
   apply Lam_typed.
-  apply App_typed with (τ1 := (TRec (TArrow (TVar 0) τ))).
+  apply App_typed with (τ1 := (TRec (TArrow (TVar 0) (TArrow τa τr)))).
   - apply Lam_typed.
-    apply App_typed with (τ1 := τ); first by apply Var_typed.
-    apply App_typed with (τ1 := TRec (TArrow (TVar 0) τ)).
-    + apply Unfold_typed_help_2 with (τ := TArrow (TVar 0) τ).
-      asimpl. by rewrite P. by apply Var_typed.
-    + by apply Var_typed.
-  - apply Fold_typed. asimpl. rewrite P.
+    apply App_typed with (τ1 := TArrow τa τr); first by apply Var_typed.
     apply Lam_typed.
-    apply App_typed with (τ1 := τ); first by apply Var_typed.
-    apply App_typed with (τ1 := TRec (TArrow (TVar 0) τ)).
-    + apply Unfold_typed_help_2 with (τ := (TArrow (TVar 0) τ)).
-      asimpl. by rewrite P. by apply Var_typed.
+    apply App_typed with (τ1 := τa).
+    + apply App_typed with (τ1 := TRec (TArrow (TVar 0) (TArrow τa τr))).
+      apply Unfold_typed_help_2 with (τ := TArrow (TVar 0) (TArrow τa τr)).
+      asimpl. by rewrite pa pr. by apply Var_typed. by apply Var_typed.
+    + by apply Var_typed.
+  - apply Fold_typed. asimpl. rewrite pa pr.
+    apply Lam_typed.
+    apply App_typed with (τ1 := (TArrow τa τr)); first by apply Var_typed.
+    apply Lam_typed.
+    apply App_typed with (τ1 := τa).
+    apply App_typed with (τ1 := TRec (TArrow (TVar 0) (TArrow τa τr))).
+    apply Unfold_typed_help_2 with (τ := TArrow (TVar 0) (TArrow τa τr)).
+    asimpl. by rewrite pa pr. by apply Var_typed. by apply Var_typed.
+    by apply Var_typed.
+Qed.
+
+(* avoid to much substitutions since autosubst is as slow as a snail *)
+
+Definition Fix' (f : expr) : expr :=
+  (Lam ((rename (+1) f) (Lam ((Unfold (Var 1)) (Var 1) (Var 0)))))
+    (Fold (Lam (rename (+1) f (Lam ((Unfold (Var 1)) (Var 1) (Var 0)))))).
+
+Lemma Fix'_typed Γ τa τr f (pa : Is_Closed τa) (pr : Is_Closed τr) :
+  (Γ ⊢ₛ f : (TArrow (TArrow τa τr) (TArrow τa τr))) -> (Γ ⊢ₛ Fix' f : (TArrow τa τr)).
+Proof.
+  intros H.
+  apply App_typed with (τ1 := (TRec (TArrow (TVar 0) (TArrow τa τr)))).
+  - apply Lam_typed.
+    apply App_typed with (τ1 := TArrow τa τr). asimpl. rewrite -rename_ren. apply up_type_one. apply H.
+    apply Lam_typed.
+    apply App_typed with (τ1 := τa).
+    + apply App_typed with (τ1 := TRec (TArrow (TVar 0) (TArrow τa τr))).
+      asimpl. apply Unfold_typed_help_2 with (τ := TArrow (TVar 0) (TArrow τa τr)).
+      asimpl. by rewrite pa pr. by apply Var_typed. by apply Var_typed.
+    + by apply Var_typed.
+  - apply Fold_typed. asimpl. rewrite pa pr.
+    apply Lam_typed.
+    apply App_typed with (τ1 := (TArrow τa τr)). rewrite -rename_ren. apply up_type_one. apply H.
+    apply Lam_typed.
+    apply App_typed with (τ1 := τa).
+    apply App_typed with (τ1 := TRec (TArrow (TVar 0) (TArrow τa τr))).
+    + apply Unfold_typed_help_2 with (τ := (TArrow (TVar 0) (TArrow τa τr))).
+      asimpl. by rewrite pa pr. by apply Var_typed.
+    + by apply Var_typed.
     + by apply Var_typed.
 Qed.
+
+Lemma Fix'_subs_rewrite f σ : (Fix' f).[σ] = Fix' (f.[σ]).
+Proof.
+  rewrite /Fix'.
+  by asimpl.
+Qed.
+
+Definition Fix'' (f : expr) : expr :=
+  (Unfold (Fold (Lam ((rename (+1) f) (Lam ((Unfold (Var 1)) (Var 1) (Var 0)))))))
+    (Fold (Lam (rename (+1) f (Lam ((Unfold (Var 1)) (Var 1) (Var 0)))))).
+
+Lemma Fix''_typed Γ τa τr f (pa : Is_Closed τa) (pr : Is_Closed τr) :
+  (Γ ⊢ₛ f : (TArrow (TArrow τa τr) (TArrow τa τr))) -> (Γ ⊢ₛ Fix'' f : (TArrow τa τr)).
+Proof.
+  intros H.
+  apply App_typed with (τ1 := (TRec (TArrow (TVar 0) (TArrow τa τr)))).
+  - apply Unfold_typed_help_2 with (τ := TArrow (TVar 0) (TArrow τa τr)). by asimpl; by rewrite pa pr.
+    apply Fold_typed.
+    apply Lam_typed.
+    apply App_typed with (τ1 := TArrow τa τr). asimpl. rewrite -rename_ren. apply up_type_one.
+    rewrite pa pr.
+    apply H.
+    apply Lam_typed.
+    apply App_typed with (τ1 := τa).
+    + apply App_typed with (τ1 := TRec (TArrow (TVar 0) (TArrow τa τr))).
+      asimpl. apply Unfold_typed_help_2 with (τ := TArrow (TVar 0) (TArrow τa τr)).
+      asimpl. by rewrite pa pr. by apply Var_typed. by apply Var_typed.
+    + by apply Var_typed.
+  - apply Fold_typed. asimpl. rewrite pa pr.
+    apply Lam_typed.
+    apply App_typed with (τ1 := (TArrow τa τr)). rewrite -rename_ren. apply up_type_one. apply H.
+    apply Lam_typed.
+    apply App_typed with (τ1 := τa).
+    apply App_typed with (τ1 := TRec (TArrow (TVar 0) (TArrow τa τr))).
+    + apply Unfold_typed_help_2 with (τ := (TArrow (TVar 0) (TArrow τa τr))).
+      asimpl. by rewrite pa pr. by apply Var_typed.
+    + by apply Var_typed.
+    + by apply Var_typed.
+Qed.
+
+Lemma Fix''_subs_rewrite f σ : (Fix'' f).[σ] = Fix'' (f.[σ]).
+Proof.
+  rewrite /Fix''.
+  by asimpl.
+Qed.
+
+(* Definition Fix'' (f : expr) : expr := *)
+(*   (Lam (f (Lam ((Unfold (Var 1)) (Var 1) (Var 0))))) *)
+(*     (Fold (Lam (f (Lam ((Unfold (Var 1)) (Var 1) (Var 0)))))). *)
+
+(* (* Lemma Fix''_typed Γ τa τr f (pa : Is_Closed τa) (pr : Is_Closed τr) : *) *)
+(* (*   (Γ ⊢ₛ f : (TArrow (TArrow τa τr) (TArrow τa τr))) -> (Γ ⊢ₛ Fix'' f : (TArrow τa τr)). *) *)
+(* (* Proof. *) *)
+(* (*   intros H. *) *)
+(* (*   apply App_typed with (τ1 := (TRec (TArrow (TVar 0) (TArrow τa τr)))). *) *)
+(* (*   - apply Lam_typed. *) *)
+(* (*     apply App_typed with (τ1 := TArrow τa τr). asimpl. rewrite -rename_ren. apply up_type_one. apply H. *) *)
+(* (*     apply Lam_typed. *) *)
+(* (*     apply App_typed with (τ1 := τa). *) *)
+(* (*     + apply App_typed with (τ1 := TRec (TArrow (TVar 0) (TArrow τa τr))). *) *)
+(* (*       asimpl. apply Unfold_typed_help_2 with (τ := TArrow (TVar 0) (TArrow τa τr)). *) *)
+(* (*       asimpl. by rewrite pa pr. by apply Var_typed. by apply Var_typed. *) *)
+(* (*     + by apply Var_typed. *) *)
+(* (*   - apply Fold_typed. asimpl. rewrite pa pr. *) *)
+(* (*     apply Lam_typed. *) *)
+(* (*     apply App_typed with (τ1 := (TArrow τa τr)). rewrite -rename_ren. apply up_type_one. apply H. *) *)
+(* (*     apply Lam_typed. *) *)
+(* (*     apply App_typed with (τ1 := τa). *) *)
+(* (*     apply App_typed with (τ1 := TRec (TArrow (TVar 0) (TArrow τa τr))). *) *)
+(* (*     + apply Unfold_typed_help_2 with (τ := (TArrow (TVar 0) (TArrow τa τr))). *) *)
+(* (*       asimpl. by rewrite pa pr. by apply Var_typed. *) *)
+(* (*     + by apply Var_typed. *) *)
+(* (*     + by apply Var_typed. *) *)
+(* (* Qed. *) *)
+
+(* Lemma test0 σ : (Var 0).[ids 0 .: σ] = Var 0. *)
+(* Proof. *)
+(*   by simpl. *)
+(* Qed. *)
+
+(* Lemma test1 σ : (Var 0).[ids 0 .: σ] = (Var 0). *)
+(* Proof. *)
+(*   asimpl. done. *)
+(* Qed. *)
+
+(* Lemma test2 e σ : (rename (+1) e).[ids 0 .: σ] = e.[σ]. *)
+(* Proof. *)
+(*   asimpl. done. *)
+(* Qed. *)
+
+Definition Fix_stepped : expr :=
+  (Lam (Var 1 (Lam ((Unfold (Var 1)) (Var 1) (Var 0)))))
+    (Fold (Lam (Var 1 (Lam ((Unfold (Var 1)) (Var 1) (Var 0)))))).
+
+
+Definition Fix_stepped_subs_typed Γ τa τr f (pa : Is_Closed τa) (pr : Is_Closed τr) :
+  (Γ ⊢ₛ f : (TArrow (TArrow τa τr) (TArrow τa τr))) -> (Γ ⊢ₛ Fix_stepped.[f/] : (TArrow τa τr)).
+Proof.
+  intros H.
+  apply App_typed with (τ1 := (TRec (TArrow (TVar 0) (TArrow τa τr)))).
+  - apply Lam_typed.
+    apply App_typed with (τ1 := TArrow τa τr). asimpl. rewrite -rename_ren. apply up_type_one. apply H.
+    apply Lam_typed.
+    apply App_typed with (τ1 := τa).
+    + apply App_typed with (τ1 := TRec (TArrow (TVar 0) (TArrow τa τr))).
+      asimpl. apply Unfold_typed_help_2 with (τ := TArrow (TVar 0) (TArrow τa τr)).
+      asimpl. by rewrite pa pr. by apply Var_typed. by apply Var_typed.
+    + by apply Var_typed.
+  - apply Fold_typed. asimpl. rewrite pa pr.
+    apply Lam_typed.
+    apply App_typed with (τ1 := (TArrow τa τr)). rewrite -rename_ren. apply up_type_one. apply H.
+    apply Lam_typed.
+    apply App_typed with (τ1 := τa).
+    apply App_typed with (τ1 := TRec (TArrow (TVar 0) (TArrow τa τr))).
+    + apply Unfold_typed_help_2 with (τ := (TArrow (TVar 0) (TArrow τa τr))).
+      asimpl. by rewrite pa pr. by apply Var_typed.
+    + by apply Var_typed.
+    + by apply Var_typed.
+Qed.
+
+(* Definition Fix_stepped_typed Γ τ : (Is_Closed τ) -> (((TArrow τ τ) :: Γ) ⊢ₛ Fix_stepped : τ). *)
+(* Proof. *)
+(*   intro P. *)
+(*   apply App_typed with (τ1 := (TRec (TArrow (TVar 0) τ))). *)
+(*   - apply Lam_typed. *)
+(*     apply App_typed with (τ1 := τ); first by apply Var_typed. *)
+(*     apply App_typed with (τ1 := TRec (TArrow (TVar 0) τ)). *)
+(*     + apply Unfold_typed_help_2 with (τ := TArrow (TVar 0) τ). *)
+(*       asimpl. by rewrite P. by apply Var_typed. *)
+(*     + by apply Var_typed. *)
+(*   - apply Fold_typed. asimpl. rewrite P. *)
+(*     apply Lam_typed. *)
+(*     apply App_typed with (τ1 := τ); first by apply Var_typed. *)
+(*     apply App_typed with (τ1 := TRec (TArrow (TVar 0) τ)). *)
+(*     + apply Unfold_typed_help_2 with (τ := (TArrow (TVar 0) τ)). *)
+(*       asimpl. by rewrite P. by apply Var_typed. *)
+(*     + by apply Var_typed. *)
+(* Qed. *)
