theories/refinements/static_gradual/compat_cast/all.v
@@ -1,0 +1,545 @@
+From fae_gtlc_mu.refinements.static_gradual Require Export tactics_left logical_relation resources_right compat_easy help_left compat_cast.defs.
+From fae_gtlc_mu.cast_calculus Require Export types typing.
+From fae_gtlc_mu.stlc_mu Require Export lang.
+From fae_gtlc_mu.cast_calculus Require Export lang.
+From iris.algebra Require Import list.
+From iris.proofmode Require Import tactics.
+From iris.program_logic Require Import lifting.
+From fae_gtlc_mu.cast_calculus Require Export types.
+From fae_gtlc_mu.cast_calculus Require Export consistency.structural.definition.
+From fae_gtlc_mu.backtranslation Require Export cast_help.general cast_help.extract cast_help.embed.
+
+Section compat_cast_all.
+  Context `{!heapG Σ,!gradRN Σ}.
+  Notation D := (prodO stlc_mu.lang.valO cast_calculus.lang.valO -n> iPropO Σ).
+  (* Implicit Types e : stlc_mu.lang.expr. *)
+  (* Implicit Types e : stlc_mu.lang.expr. *)
+  Implicit Types fs : list stlc_mu.lang.val.
+  (* Implicit Types f : stlc_mu.lang.val. *)
+  Implicit Types A : list (cast_calculus.types.type * cast_calculus.types.type).
+  (* Implicit Types a : (cast_calculus.types.type * cast_calculus.types.type). *)
+  Local Hint Resolve to_of_val : core.
+  Local Hint Resolve stlc_mu.lang.to_of_val : core.
+
+  (** Proving it *)
+
+  (* Lemma rewrite_subs_app (e1 e2 : expr) σ : *)
+  (*   (App e1 e2).[σ] = App e1.[σ] e2.[σ]. *)
+  (* Proof. *)
+  (*     by simpl. *)
+  (* Qed. *)
+
+ Lemma wp_fix'' (f : stlc_mu.lang.expr) Φ :
+   (▷ ▷ WP f (stlc_mu.lang.Lam (rename (+1) (Fix'' f) (stlc_mu.lang.Var 0)))   {{ Φ }} -∗ (WP (Fix'' f) {{ Φ }}))%I.
+ Proof.
+   iIntros "H".
+   rewrite{2} /Fix''.
+   iApply (wp_bind $ stlc_mu.lang.fill_item $ stlc_mu.lang.AppLCtx _).
+   apply (@ectxi_lang_ctx_item stlc_mu.lang.ectxi_lang). (* hmmmm :( *)
+   wp_head.
+   (* iApply wp_pure_step_later; auto; iNext. *)
+   iApply wp_value.
+   simpl.
+   iApply wp_pure_step_later; auto; iNext.
+   asimpl.
+   iApply "H".
+ Qed.
+
+  Lemma refold_interp_unknown' vv' : fixpoint interp_unknown1' vv' ≡ interp TUnknown [] vv'.
+  Proof.
+    auto.
+  Qed.
+
+  Lemma back_cast_ar_all {A} {τi τf} (pC : cons_struct A τi τf) : back_cast_ar pC.
+  Proof.
+    induction pC; rewrite /𝓕c /𝓕 /back_cast_ar; iIntros (ei' K' v v' fs) "(#Hfs & #Hvv' & #Hei' & Hv')".
+    - rewrite /𝓕c /𝓕 extract_no_subs.
+      destruct G.
+      + (** TUnit *) rewrite unfold_fixpoint_interp_unknown1'.
+        iDestruct "Hvv'" as "[Hvv'Unit|[Hpp'|[Hss'|[Hff'|Huu']]]]".
+        * iDestruct "Hvv'Unit" as "%"; inversion H; clear v v' H H1 H2.
+          admit.
+        * iDestruct "Hpp'" as (v1 v1' v2 v2') "(% & #H1 & #H2)". simpl in H; inversion H; clear H H1 H2 v v'.
+          repeat rewrite (refold_interp_unknown').
+          admit.
+        * iDestruct "Hss'" as "[H1 | H2]".
+          -- iDestruct "H1" as (v1 v1') "[% Hv1v1']"; rewrite (refold_interp_unknown'); inversion H; clear H H1 H2 v v'.
+             admit.
+          -- iDestruct "H2" as (v2 v2') "[% Hv2v2']"; rewrite (refold_interp_unknown'); inversion H; clear H H1 H2 v v'.
+             admit.
+        * iDestruct "Hff'" as (f f') "[% Hff']". inversion H. clear H H1 H2 v v'.
+          admit.
+        * iDestruct "Huu'" as (u u') "[% H]"; rewrite (refold_interp_unknown'); inversion H; clear H H1 H2 v v'.
+          admit.
+        * constructor.
+      + (** TProd *) admit.
+      + (** TSum *) admit.
+      + (** TArrow *) rewrite unfold_fixpoint_interp_unknown1'.
+        iDestruct "Hvv'" as "[Hvv'Unit|[Hpp'|[Hss'|[Hff'|Huu']]] ]".
+        * iDestruct "Hvv'Unit" as "%"; inversion H; clear v v' H H1 H2.
+          admit.
+        * iDestruct "Hpp'" as (v1 v1' v2 v2') "(% & #H1 & #H2)". simpl in H; inversion H; clear H H1 H2 v v'.
+          repeat rewrite (refold_interp_unknown').
+          admit.
+        * iDestruct "Hss'" as "[H1 | H2]".
+          -- iDestruct "H1" as (v1 v1') "[% Hv1v1']"; rewrite (refold_interp_unknown'); inversion H; clear H H1 H2 v v'.
+             admit.
+          -- iDestruct "H2" as (v2 v2') "[% Hv2v2']"; rewrite (refold_interp_unknown'); inversion H; clear H H1 H2 v v'.
+             admit.
+        * iDestruct "Hff'" as (f f') "[% Hff']". inversion H. clear H H1 H2 v v'.
+          admit.
+        * iDestruct "Huu'" as (u u') "[% H]"; rewrite (refold_interp_unknown'); inversion H; clear H H1 H2 v v'.
+          admit.
+        * constructor.
+      + (** TRec *) rewrite unfold_fixpoint_interp_unknown1'.
+        iDestruct "Hvv'" as "[Hvv'Unit|[Hpp'|[Hss'|[Hff'|Huu']]] ]".
+        * iDestruct "Hvv'Unit" as "%"; inversion H; clear v v' H H1 H2.
+          admit.
+        * iDestruct "Hpp'" as (v1 v1' v2 v2') "(% & #H1 & #H2)". simpl in H; inversion H; clear H H1 H2 v v'.
+          repeat rewrite (refold_interp_unknown').
+          admit.
+        * iDestruct "Hss'" as "[H1 | H2]".
+          -- iDestruct "H1" as (v1 v1') "[% Hv1v1']"; rewrite (refold_interp_unknown'); inversion H; clear H H1 H2 v v'.
+             admit.
+          -- iDestruct "H2" as (v2 v2') "[% Hv2v2']"; rewrite (refold_interp_unknown'); inversion H; clear H H1 H2 v v'.
+             admit.
+        * iDestruct "Hff'" as (f f') "[% Hff']". inversion H. clear H H1 H2 v v'.
+          admit.
+        * iDestruct "Huu'" as (u u') "[% H]"; rewrite (refold_interp_unknown'); inversion H; clear H H1 H2 v v'.
+          admit.
+        * constructor.
+    - rewrite /𝓕c /𝓕. rewrite embed_no_subs. destruct G.
+      + iDestruct "Hvv'" as "%". simpl in H. inversion H. rewrite H0 H1. clear v v' H H0 H1.
+        admit.
+      + iDestruct "Hvv'" as ((v1 , v1') (v2 , v2')) "[% [H1 H2]]". simpl in H; inversion H; clear H H1 H2 v v'.
+        admit.
+      + iDestruct "Hvv'" as "[H1 | H2]".
+        * iDestruct "H1" as ((v1 , v1')) "[% H1]".
+          simpl in H; inversion H; clear H H1 H2 v v'.
+          admit.
+        * iDestruct "H2" as ((v2 , v2')) "[% H2]".
+          simpl in H; inversion H; clear H H1 H2 v v'.
+          admit.
+      + admit.
+      + admit.
+    - admit.
+    - admit.
+    - admit.
+    - admit.
+    - admit.
+    - admit.
+    - fold interp.
+      rename v into f. rename v' into f'. iDestruct "Hv'" as "Hf'". iDestruct "Hvv'" as "Hff'". iClear "Hvv'".
+      rewrite /𝓕c /𝓕.
+      fold (𝓕 pC1) (𝓕 pC2).
+      rewrite between_TArrow_subst_rewrite.
+      fold (𝓕c pC1 fs) (𝓕c pC2 fs).
+      iDestruct "Hfs" as "[% Hfs']"; iAssert (rel_cast_functions A fs) with "[Hfs']" as "Hfs". iSplit; done. iClear "Hfs'".
+      do 2 rewrite 𝓕c_rewrite.
+      unfold between_TArrow.
+      wp_head.
+      asimpl.
+      iApply wp_value.
+      iExists (CastV f' (TArrow τ1 τ2) (TArrow τ3 τ4) (Between_arrow_types τ1 τ2 τ3 τ4)).
+      iSplitL "Hf'"; first done.
+      iModIntro.
+      (** actual thing to prove *)
+      (** ===================== *)
+      iIntros ((a , a')) "#Haa'".
+      simpl. clear K'.
+      iIntros (K') "Hf'".
+      simpl in *.
+      (** implementation *)
+      wp_head. asimpl.
+      (** specification *)
+      iMod (step_pure _ ei' K'
+                      (App (Cast (# f') (TArrow τ1 τ2) (TArrow τ3 τ4)) (# a'))
+                      (Cast (App (# f') (Cast (# a') τ3 τ1)) τ2 τ4) with "[Hf']") as "Hf'".
+      intros. eapply AppCast; try by rewrite -to_of_val. auto. by iFrame.
+      (** first IH for the arguments *)
+      iApply (wp_bind (fill $ [stlc_mu.lang.AppRCtx _ ; stlc_mu.lang.AppRCtx _])).
+      iApply (wp_wand with "[-]").
+      rewrite -𝓕c_rewrite.
+      iApply (IHpC1 ei' (AppRCtx f' :: CastCtx τ2 τ4 :: K') with "[Hf']").
+      (* iApply (IHpC1 ei' (CastCtx τ2 τ4 :: AppRCtx f' :: K') with "[Hf']"). *)
+      iSplitR. done.
+      iSplitR. done.
+      iSplitR. done.
+      simpl. done.
+      iIntros (b) "HHH".
+      iDestruct "HHH" as (b') "[Hb' #Hbb']".
+      simpl.
+      iClear "Haa'". clear a a'.
+      (** using the relatedness of functions *)
+      iApply (wp_bind (fill $ [stlc_mu.lang.AppRCtx _ ])).
+      iDestruct "Hff'" 
+      iApply (wp_wand with "[-]").
+      iApply ("Hff' (b , b') " with "[]").
+
+      iApply ()
+
+      iApply wp
+      iApply (wp_wand with "[-]").
+      
+      admit.
+      admit.
+
+
+      (* iApply (IHpC ei' (FoldCtx :: K') w w' (𝓕cV (consTRecTRecExposeCall A τl τr pμτlμτrnotA pC) fs H :: fs)). iSplitL "Hfs". iSplitR; first by done. *)
+
+
+
+
+      (* iIntros  *)
+
+
+
+
+    - (** setting up iLöb *)
+      (* iLöb as "IHlob" forall (v v' ei') "Hvv' Hei'". *)
+      fold (𝓕c (consTRecTRecExposeCall A τl τr pμτlμτrnotA pC) fs).
+      (* iRevert (ei' K' v v') "Hvv' Hei' Hv'". *)
+      rewrite /𝓕c /𝓕.
+      fold (𝓕 pC).
+      (** rewriting value relation for v and v' *)
+      rewrite fixpoint_interp_rec1_eq.
+      iDestruct "Hvv'" as ([w w']) "#[% Hww']".
+      inversion H; clear v v' H H1 H2.
+      fold interp.
+      fold (interp_rec ⟦ τl ⟧ []).
+      assert (bydef : interp_rec ⟦ τl ⟧ [] = ⟦ TRec τl ⟧ []); auto; rewrite bydef. clear bydef.
+      rewrite (interp_subst [] τl (TRec τl) (w, w')).
+      (** evaluation steps in WP *)
+      (* applying to value v *)
+      iApply wp_pure_step_later; auto; iNext.
+      (* bringing subs of fs inwards *)
+      rewrite rewrite_subs_app.
+      do 2 rewrite Fix''_subs_rewrite.
+      asimpl.
+      (* evaluation step of the Fix'' itself *)
+      iApply (wp_bind (stlc_mu.lang.fill_item $ stlc_mu.lang.AppLCtx _)).
+      iApply wp_fix''.
+      (** easy steps *)
+      iApply wp_pure_step_later; auto; iNext.
+      do 2 iNext.
+      iApply wp_value.
+      iApply wp_pure_step_later; auto; iNext. (* unfold fold w *)
+      (** rewriting *)
+      asimpl.
+      assert (H :
+                (stlc_mu.lang.Lam
+                   (stlc_mu.lang.Unfold
+                      (stlc_mu.lang.Fold
+                         (stlc_mu.lang.Lam
+                            (stlc_mu.lang.Lam
+                               (stlc_mu.lang.Lam
+                                  (stlc_mu.lang.Fold
+                                     ((𝓕 pC).[ids 1
+                                                  .: stlc_mu.typing.env_subst fs >>
+                                                  ren (+4)]
+                                               (stlc_mu.lang.Unfold (ids 0)))))
+                               (stlc_mu.lang.Lam
+                                  (stlc_mu.lang.Unfold (ids 1) (ids 1) (ids 0))))))
+                      (stlc_mu.lang.Fold
+                         (stlc_mu.lang.Lam
+                            (stlc_mu.lang.Lam
+                               (stlc_mu.lang.Lam
+                                  (stlc_mu.lang.Fold
+                                     ((𝓕 pC).[ids 1
+                                                  .: stlc_mu.typing.env_subst fs >>
+                                                  ren (+4)]
+                                               (stlc_mu.lang.Unfold (ids 0)))))
+                               (stlc_mu.lang.Lam
+                                  (stlc_mu.lang.Unfold (ids 1) (ids 1) (ids 0))))))
+                      (ids 0)) = (between_TRec' (𝓕 pC)).[stlc_mu.typing.env_subst fs] )
+             ). by asimpl. rewrite H; clear H.
+      rewrite between_TRec'_subst_rewrite.
+      rewrite between_TRec'_to_value.
+      assert (H : (𝓕 pC).[stlc_mu.lang.of_val (between_TRecV' (𝓕 pC).[up (stlc_mu.typing.env_subst fs)]) .: stlc_mu.typing.env_subst fs] = (𝓕 pC).[stlc_mu.typing.env_subst (between_TRecV' (𝓕 pC).[up (stlc_mu.typing.env_subst fs)] :: fs)]); first by simpl. rewrite H; clear H.
+      (** easy steps *)
+      iApply (wp_bind (stlc_mu.lang.fill_item $ stlc_mu.lang.FoldCtx)).
+      iDestruct "Hfs" as "[% Hfs']"; iAssert (rel_cast_functions A fs) with "[Hfs']" as "Hfs". iSplit; done.
+      (* iDestruct "Hfs" as "[% Hfs]". *)
+      assert (Hs : length ((TRec τl, TRec τr) :: A) =
+                  length
+                    (between_TRecV'
+                       (𝓕 pC).[up (stlc_mu.typing.env_subst fs)] :: fs)). simpl; auto.
+      fold (𝓕c pC (between_TRecV' (𝓕 pC).[up (stlc_mu.typing.env_subst fs)] :: fs)).
+      (* fold (𝓕c (consTRecTRecExposeCall A τl τr pμτlμτrnotA pC) fs). *)
+      rewrite 𝓕c_rewrite.
+      iApply (wp_bind (stlc_mu.lang.fill_item $ stlc_mu.lang.AppRCtx _)).
+      iApply wp_pure_step_later; auto; iNext.
+      iApply wp_value.
+      simpl. (** hmmm; unfolds IHLöb... *)
+      (** rewriting stuff *)
+      rewrite -𝓕c_rewrite /𝓕c.
+      assert (T : between_TRecV' (𝓕 pC).[up (stlc_mu.typing.env_subst fs)] =
+                  (𝓕cV (consTRecTRecExposeCall A τl τr pμτlμτrnotA pC) fs H)
+             ). {
+        apply stlc_mu.lang.of_val_inj.
+        rewrite -between_TRec'_to_value.
+        rewrite -between_TRec'_subst_rewrite.
+        by simpl.
+        (* rewrite -𝓕c_rewrite. rewrite /𝓕c. *)
+        (* by simpl. *)
+      } rewrite T. clear T.
+      (** eval specification side *)
+      iMod (step_pure _ ei' K'
+                      (Cast (Fold w') (TRec τl) (TRec τr))
+                      (Fold (Cast (Unfold (Fold w')) (τl.[TRec τl/]) (τr.[TRec τr/]))) with "[Hv']") as "Hv'".
+      intros. apply (RecursiveCast _ (FoldV w')). by rewrite -to_of_val. auto. by iFrame.
+      iMod (step_pure _ ei' (CastCtx τl.[TRec τl/] τr.[TRec τr/] :: FoldCtx :: K')
+                      (Unfold (Fold (# w')))
+                      w' with "[Hv']") as "Hv'".
+      intros. apply (Unfold_Fold _ w'). by rewrite to_of_val. auto. by iFrame.
+      (** apply IH *)
+      iApply (wp_wand with "[-]").
+      iApply (IHpC ei' (FoldCtx :: K') w w' (𝓕cV (consTRecTRecExposeCall A τl τr pμτlμτrnotA pC) fs H :: fs)). iSplitL "Hfs". iSplitR; first by done.
+      (** applying IHlob and Hfs *)
+      admit.
+      (** other *)
+      iSplitR. done. iSplitR. done. by simpl.
+      (** finish *)
+      iIntros (v) "H".
+      iDestruct "H" as (v') "[Hv' #Hvv']".
+      iApply wp_value.
+      iExists (FoldV v').
+      iFrame.
+      rewrite fixpoint_interp_rec1_eq.
+      simpl. iModIntro.
+      iExists (v , v').
+      iSplitR. done.
+      iNext.
+      by rewrite (interp_subst [] τr (TRec τr) (v, v')).
+    - 
+      rewrite /𝓕c /𝓕. asimpl.
+      (** getting the information about the length of the list *)
+      iDestruct "Hfs" as "[% Hfs']".
+      (* iAssert (rel_cast_functions A fs) with "[Hfs']" as "Hfs". iSplit; done. *)
+
+      destruct (fs !! i) as [f | abs] eqn:Hf.
+      + simpl.
+        rewrite (stlc_mu.typing.env_subst_lookup _ i f); try done.
+        iDestruct (big_sepL_lookup_acc _  i with "Hfs'") as "HHHH". apply Hf.
+
+
+        iDestruct (big_sepL_lookup_acc (∀ (v0 : stlc_mu.lang.val) (v'0 : val),
+            ⟦ TRec τl ⟧ [] (v0, v'0) → ⟦ TRec τr ⟧ₑ [] (f ( v0), Cast (# v'0) (TRec τl) (TRec τr))) _ i with "Hfs'") as "HHHH". apply Hf.
+
+j/sep
+        jkjjk
+
+
+      + assert (Hi : i < length fs). rewrite -H. by eapply lookup_lt_Some.
+        assert (Hi' : i >= length fs). by apply lookup_ge_None_1. exfalso. lia.
+
+
+  Admitted.
+
+
+
+
+
+
+        fold interp_unknown1 interp_unknown.
+        rewrite interp_unknown_unfold /interp_unknown1; iDestruct "Hvv'" as "#Hvv'"; iDestruct "Hvv'" as "[Hvv'Unit|[Hpp'|[Hss'|[Hff'|Hur']]] ]"; fold interp_unknown1 interp_unknown.
+        * iDestruct "Hvv'Unit" as ((w , w')) "[% Hww']"; simpl in H; inversion H; clear v v' H H1 H2.
+          asimpl.
+          iApply wp_pure_step_later; auto; iNext; asimpl.
+          iDestruct "Hww'" as "%"; inversion H; rewrite H0 H1; clear w w' H H0 H1.
+          iApply (wp_bind (stlc_mu.lang.fill_item $ stlc_mu.lang.CaseCtx _ _)).
+          iApply wp_pure_step_later; auto; iNext.
+          iApply wp_value.
+          iApply wp_pure_step_later; auto; iNext.
+          iApply wp_pure_step_later; auto; iNext. asimpl.
+          iApply wp_pure_step_later; auto; iNext.
+          iApply wp_pure_step_later; auto; iNext. asimpl.
+          iMod (step_pure _ ei' K' (Cast (Cast Unit TUnit ⋆) ⋆ TUnit) (# UnitV) with "[Hv']") as "HHHH"; intros; auto.
+          apply Same_Ground with (v := UnitV ); auto; constructor.
+          iApply wp_value.
+          iExists UnitV.
+          by repeat iFrame.
+        * (* diverging branch *)
+          iDestruct "Hpp'" as ((p , p')) "[% Hpp']"; simpl in H; inversion H; clear H H1 H2 v v'.
+          asimpl.
+          iApply wp_pure_step_later; auto; iNext; asimpl.
+          iDestruct "Hpp'" as ((v1 , v1') (v2 , v2')) "[% [Hv1v1' Hv2v2']]"; simpl in H; inversion H; clear H H1 H2 p p'.
+          iApply (wp_bind (stlc_mu.lang.fill_item $ stlc_mu.lang.CaseCtx _ _)).
+          iApply wp_pure_step_later; auto; iNext.
+          iApply wp_value.
+          iApply wp_pure_step_later; auto; iNext; asimpl.
+          iApply wp_pure_step_later; auto; iNext; asimpl.
+          iApply wp_pure_step_later; auto; iNext. asimpl.
+          by iApply wp_Ω.
+        * admit.
+        * admit.
+        * iDestruct "Hur'" as ((u , r')) "[% Hr]". simpl in H. inversion H. clear H H1 H2.
+          admit.
+      + rewrite interp_unknown_unfold /interp_unknown1; iDestruct "Hvv'" as "#Hvv'"; iDestruct "Hvv'" as "[Hvv'Unit|[Hpp'|[Hss'|[Hff'|Hur']]] ]"; fold interp_unknown1 interp_unknown.
+        * (* diverging branch *)
+          iDestruct "Hvv'Unit" as ((w , w')) "[% Hww']"; simpl in H; inversion H; clear v v' H H1 H2.
+          asimpl.
+          iApply wp_pure_step_later; auto; iNext; asimpl.
+          iDestruct "Hww'" as "%"; inversion H; rewrite H0 H1; clear w w' H H0 H1.
+          iApply (wp_bind (stlc_mu.lang.fill_item $ stlc_mu.lang.CaseCtx _ _)).
+          iApply wp_pure_step_later; auto; iNext.
+          iApply wp_value.
+          iApply (wp_bind (stlc_mu.lang.fill_item $ stlc_mu.lang.CaseCtx _ _)).
+          iApply wp_value.
+          iApply wp_pure_step_later; auto; iNext.
+          iApply wp_pure_step_later; auto; iNext. asimpl.
+          iApply wp_pure_step_later; auto; iNext. asimpl.
+          by iApply wp_Ω.
+        * iDestruct "Hpp'" as ((p , p')) "[% Hpp']"; simpl in H; inversion H; clear H H1 H2.
+          asimpl.
+          iApply wp_pure_step_later; auto; iNext; asimpl.
+          iDestruct "Hpp'" as ((v1 , v1') (v2 , v2')) "[% [Hv1v1' Hv2v2']]"; simpl in H; inversion H; clear H H1 H2 p p'.
+          iApply (wp_bind (stlc_mu.lang.fill_item $ stlc_mu.lang.CaseCtx _ _)).
+          iApply wp_pure_step_later; auto; iNext.
+          iApply wp_value.
+          iApply wp_pure_step_later; auto; iNext; asimpl.
+          iApply wp_pure_step_later; auto; iNext; asimpl.
+          iApply wp_pure_step_later; auto; iNext. asimpl.
+          iMod (step_pure _ ei' K'
+                          (Cast
+                             (Cast (Pair (# v1') (# v2'))
+                                   (⋆ × ⋆) ⋆) ⋆
+                             (⋆ × ⋆)
+                          )
+                          (Pair (# v1') (# v2'))
+                  with "[Hv']") as "HHHH"; auto.
+          intro. eapply Same_Ground. simplify_option_eq. auto. constructor.
+          iApply wp_value.
+          iExists (PairV (v1') (v2')).
+          simpl. repeat iFrame.
+          iExists (v1 , v1') , (v2 , v2'). by auto.
+        * admit.
+        * admit.
+        * admit.
+      + admit.
+      + admit.
+      + rewrite interp_unknown_unfold /interp_unknown1; iDestruct "Hvv'" as "#Hvv'"; iDestruct "Hvv'" as "[Hvv'Unit|[Hpp'|[Hss'|[Hff'|Hur']]] ]"; fold interp_unknown1 interp_unknown.
+        * admit.
+        * admit.
+        * admit.
+        * admit.
+        * iDestruct "Hur'" as ((u , r')) "[% Hur']"; inversion H; clear H H1 H2.
+          iMod (step_pure _ ei' K'
+                          (Cast (# castupV_TRec r') ⋆ (TRec ⋆))
+                          (# r')
+                  with "[Hv']") as "HHHH"; auto.
+          intro; eapply Same_Ground; simplify_option_eq; auto; constructor.
+          iApply wp_pure_step_later; auto; iNext; asimpl.
+          iApply (wp_bind (stlc_mu.lang.fill_item $ stlc_mu.lang.CaseCtx _ _)).
+          iApply wp_pure_step_later; auto.
+          iApply wp_value. simpl. 
+          iApply wp_pure_step_later; auto. asimpl. 
+          iApply wp_value.
+          repeat iNext.
+          iExists r'. by iFrame.
+    - destruct G; rewrite /𝓕c /𝓕.
+      + iApply wp_pure_step_later; auto; iNext; asimpl.
+        iDestruct "Hvv'" as "%"; inversion H. rewrite H0 H1. clear H H0 H1 v v'.
+        iApply wp_value. iExists (CastV UnitV TUnit ⋆ (From_ground_to_unknown TUnit Ground_TUnit)).
+        simpl in *.
+        iFrame.
+        rewrite interp_unknown_unfold /interp_unknown1.
+        admit.
+      + admit.
+      + admit.
+      + admit.
+      + rewrite fixpoint_interp_rec1_eq.
+        iDestruct "Hvv'" as ((r , r')) "[% #Hrr']". inversion H; clear H H1 H2.
+        iApply wp_pure_step_later; auto; iNext; asimpl.
+        iApply (wp_bind (fill [stlc_mu.lang.InjRCtx ; stlc_mu.lang.FoldCtx ])).
+        iApply wp_pure_step_later; auto. iNext; asimpl.
+        iApply wp_value.
+        iApply wp_value.
+        iExists (CastV (FoldV r') (TRec ⋆) ⋆ (From_ground_to_unknown (TRec ⋆) Ground_TRec)).
+        simpl in *.
+        iFrame.
+        rewrite{1} interp_unknown_unfold.
+        rewrite{1} interp_unknown_unfold.
+        repeat rewrite{1} /interp_unknown1.
+        iRight.
+        iRight.
+        iRight.
+        iRight.
+        iModIntro.
+        iExists (r , FoldV r'). simpl. iSplitL.
+        auto.
+        admit.
+    - admit.
+    - admit.
+    - rewrite /𝓕c /𝓕. asimpl.
+      iApply wp_pure_step_later; auto.
+      asimpl.
+      iDestruct "Hvv'" as %[eq1 eq2]; simplify_eq.
+      iNext.
+      iMod (step_pure _ ei' K' (Cast (# UnitV) TUnit TUnit) (# UnitV) with "[Hv']") as "HHHH"; auto.
+      intros; by eapply IdBase.
+      iApply wp_value.
+      iExists UnitV. iFrame. iSplit; trivial.
+    - rewrite /𝓕c /𝓕; asimpl.
+      iMod (step_pure _ ei' K' (Cast (# v') ⋆ ⋆) (# v') with "[Hv']") as "Hv'"; auto.
+      intros; by eapply IdStar.
+      iApply wp_pure_step_later; auto; asimpl.
+      iNext.
+      iApply wp_value.
+      iExists v'. iFrame.
+    - iDestruct "Hvv'" as "[Hvv'1 | Hvv'2]".
+      + iDestruct "Hvv'1" as (vv'1) "Hvv'1". destruct vv'1 as (v1 , v1').
+        iDestruct "Hvv'1" as "[% Hvv'1]". inversion H.
+        iMod (step_pure _ ei' K' (Cast (# InjLV v1') (τ1 + τ2)%type (τ1' + τ2')%type) _ with "[Hv']") as "Hv'"; auto; try (intros; eapply SumCast; auto).
+        iMod ((step_case_inl _ ei' K' (# v1')) with "[Hv']") as "Hv'"; auto.
+        (* rewrite /𝓕c /𝓕 /between_TSum. *)
+        rewrite /𝓕c /𝓕.
+        iApply wp_pure_step_later. auto; asimpl.
+        iApply wp_pure_step_later; auto; asimpl.
+        iNext. iNext.
+        iApply wp_bind. admit.
+        iApply wp_wand_r.
+        iSplitL.
+        iApply (IHpC1 ei' (InjLCtx :: K')). repeat iFrame. auto.
+        clear H H1 H2 v1 v1'.
+        iIntros (v1) "HHH". iDestruct "HHH" as (v1') "[Hv1' Hvv'1]".
+        iApply wp_value.
+        iExists (InjLV v1'). repeat iFrame. iLeft. iExists (v1 , v1').
+        iSplitR. by simpl. done.
+      + admit.
+    - iSimpl in "Hvv'". iDestruct "Hvv'" as ((v1 , v1') (v2 , v2')) "[% [Hv1v1' Hv2v2']]". simpl in H; inversion H; clear H H1 H2 v v'.
+      iApply wp_pure_step_later; auto.
+      fold (𝓕 pC1) (𝓕 pC2). asimpl. fold (𝓕c pC1 fs) (𝓕c pC2 fs).
+      iDestruct "Hfs" as "[% Hfs']"; iAssert (rel_cast_functions A fs) with "[Hfs']" as "Hfs". iSplit; done.
+      rewrite 𝓕c_rewrite.
+      iApply (wp_bind (fill [stlc_mu.lang.AppRCtx (𝓕cV pC1 fs H) ; stlc_mu.lang.PairLCtx ((𝓕c pC2 fs) (stlc_mu.lang.Snd (stlc_mu.lang.Pair (stlc_mu.lang.of_val v1) (stlc_mu.lang.of_val v2)))) ])).
+      iApply wp_pure_step_later; auto.
+      do 2 iNext. iApply wp_value. simpl.
+      iApply (wp_bind (fill [stlc_mu.lang.PairLCtx ((𝓕c pC2 fs) (stlc_mu.lang.Snd (stlc_mu.lang.Pair (stlc_mu.lang.of_val v1) (stlc_mu.lang.of_val v2)))) ])).
+      rewrite -𝓕c_rewrite.
+      iApply (wp_wand with "[Hfs Hv1v1' Hei' Hv']").
+      (* iApply (IHpC1 ei' :: K' with "Hfs Hv1v1' Hei' Hv'"). *)
+      admit.
+      admit.
+    - admit.
+    - rewrite /𝓕c /𝓕.
+      fold (𝓕 pC).
+      iApply wp_pure_step_later; auto; asimpl.
+      iApply (wp_bind $ stlc_mu.lang.fill_item $ stlc_mu.lang.AppLCtx _).
+      iApply wp_pure_step_later; auto; asimpl.
+      iApply wp_pure_step_later; auto; asimpl.
+
+    - rewrite /𝓕c /𝓕. asimpl.
+      destruct (fs !! i) as [f | abs] eqn:Hf.
+      + rewrite (stlc_mu.typing.env_subst_lookup _ _ f); auto.
+        iDestruct "Hfs" as "[% Hfs]".
+        rewrite fixpoint_interp_rec1_eq.
+        
+        rewrite interp_unknown_unfold /interp_unknown1.
+        unfold fixpoint_re
+        iAssert 
+        
+    destruct ()
+
+
+End compat_cast_all.
