theories/refinements/static_gradual/compat_cast/defs.v
@@ -1,0 +1,97 @@
+From fae_gtlc_mu.refinements.static_gradual Require Export logical_relation resources_right compat_easy help_left.
+From fae_gtlc_mu.cast_calculus Require Export types typing.
+From fae_gtlc_mu.stlc_mu Require Export lang.
+From fae_gtlc_mu.cast_calculus Require Export lang.
+From iris.algebra Require Import list.
+From iris.proofmode Require Import tactics.
+From iris.program_logic Require Import lifting.
+From fae_gtlc_mu.cast_calculus Require Export types.
+From fae_gtlc_mu.cast_calculus Require Export consistency.structural.definition.
+From fae_gtlc_mu.backtranslation Require Export cast_help.general cast_help.extract cast_help.embed.
+
+(* Coercion stlc_mu.lang.of_val : stlc_mu.lang.val >-> stlc_mu.lang.expr. *)
+(* Coercion cast_calculus.lang.of_val : cast_calculus.lang.val >-> cast_calculus.lang.expr. *)
+
+(* Notation "# v" := (of_val v) (at level 20). *)
+
+Section defs.
+  Context `{!heapG Σ,!gradRN Σ}.
+  Notation D := (prodO stlc_mu.lang.valO cast_calculus.lang.valO -n> iPropO Σ).
+  (* Implicit Types e : stlc_mu.lang.expr. *)
+  (* Implicit Types e : stlc_mu.lang.expr. *)
+  Implicit Types fs : list stlc_mu.lang.val.
+  (* Implicit Types f : stlc_mu.lang.val. *)
+  Implicit Types A : list (cast_calculus.types.type * cast_calculus.types.type).
+  (* Implicit Types a : (cast_calculus.types.type * cast_calculus.types.type). *)
+  Local Hint Resolve to_of_val : core.
+
+  (** We need to "close up" 𝓕 pC with functions... *)
+
+  Definition 𝓕c {A} {τi τf} (pC : cons_struct A τi τf) fs : stlc_mu.lang.expr :=
+    (𝓕 pC).[stlc_mu.typing.env_subst fs].
+
+  (** 𝓕 pC is a value after substitution *)
+
+  Lemma 𝓕c_is_value {A} {τi τf} (pC : cons_struct A τi τf) fs (H : length A = length fs) :
+    is_Some (stlc_mu.lang.to_val (𝓕c pC fs)).
+  Proof.
+    induction pC; rewrite /𝓕c; asimpl; try destruct G; try by econstructor.
+    assert (Hi : i < length fs). rewrite -H; apply lookup_lt_is_Some; by econstructor.
+    destruct (fs !! i) eqn:Hf.
+    rewrite (stlc_mu.typing.env_subst_lookup _ _ v).
+    rewrite stlc_mu.lang.to_of_val.
+    by econstructor.
+    done.
+    exfalso. assert (abs : length fs <= i). by apply lookup_ge_None. lia.
+  Qed.
+
+  Definition 𝓕cV {A} {τi τf} (pC : cons_struct A τi τf) fs (H : length A = length fs) : stlc_mu.lang.val :=
+    is_Some_proj (𝓕c_is_value pC fs H).
+
+  (** just redifine 𝓕C as value.. *)
+  Lemma 𝓕c_rewrite {A} {τi τf} (pC : cons_struct A τi τf) fs (H : length A = length fs) : 𝓕c pC fs = stlc_mu.lang.of_val (𝓕cV pC fs H).
+  Proof.
+    unfold 𝓕cV.
+    induction pC; rewrite /𝓕c; asimpl; try destruct G; try by econstructor.
+    assert (Hi : i < length fs). rewrite -H; apply lookup_lt_is_Some; by econstructor.
+    destruct (fs !! i) eqn:Hf.
+    destruct (𝓕c_is_value
+         (consTRecTRecUseCall A τl τr i pμτlμtrinA) fs H).
+    admit.
+    exfalso. assert (abs : length fs <= i). by apply lookup_ge_None. lia.
+  Admitted.
+
+  (** We will want to assume these functions to be meaningful..,
+      i.e. they properly relate to the casts happening on the right side *)
+
+  Definition rel_cast_functions A (fs : list stlc_mu.lang.val) : iProp Σ := ⌜length A = length fs⌝ ∗
+    [∗] (zip_with (fun p f =>
+    (∀ (v : stlc_mu.lang.val) (v' : cast_calculus.lang.val) ,
+      (⟦ p.1 ⟧ [] (v , v')) → (⟦ p.2 ⟧ₑ [] (((stlc_mu.lang.of_val f) (stlc_mu.lang.of_val v)) , Cast (# v') p.1 p.2)))%I)
+    A fs).
+
+  Global Instance rel_cast_functions_persistent A fs :
+    Persistent (rel_cast_functions A fs).
+  Proof.
+  Admitted.
+
+
+(* "'[∗' 'list]' x1 ; x2 ∈ l1 ; l2 , P" :=  *)
+(* big_sepL2 (fun _ x1 x2 => P) l1 l2 : bi_scope *)
+
+
+(*   big_sepL2_lookup: *)
+
+
+(*     big_sepL2_lookup: *)
+
+  (** The statement that the -- closed up -- back-translated casts behave appropriately.
+      (We redefine it here to a new statement, making it a bit more amenable for proving.) *)
+
+  Definition back_cast_ar {A} {τi τf} (pC : cons_struct A τi τf) :=
+  ∀ ei' K' v v' fs, bi_entails
+                      (rel_cast_functions A fs ∗ interp τi [] (v, v') ∗ initially_inv ei' ∗ currently_half (fill K' (Cast (# v') τi τf)))
+                      (WP (𝓕c pC fs (stlc_mu.lang.of_val v)) {{ w, ∃ w', currently_half (fill K' (# w')) ∗ interp τf [] (w, w') }})%I.
+
+
+End defs.
